Refactoring map equivalence and map inclusion

Map.v
@@ -5,7 +5,7 @@ Local Definition map' (A : Type) := string -> A. (* total map *)
 Local Definition empty' {A : Type} v : map' A := (fun _ => v).
 
 Local Definition update' {A : Type} (m : map' A) k v :=
-  fun k' => if eqb k k' then v else m k'.
+  fun k' => if string_dec k k' then v else m k'.
 
 Definition map (A : Type) := map' (option A). (* partial map *)
 
@@ -25,8 +25,8 @@ Notation "m '[' k '<==' v ']'" := (update m k v) (at level 9).
 Lemma lookup_update_eq : forall {A} (m : map A) k v,
   m[k <== v] k = Some v.
 Proof.
-  intros. unfold lookup, update, update'.
-  rewrite eqb_refl. reflexivity.
+  intros. unfold lookup, update, update'. eauto.
+  destruct string_dec; trivial; contradiction.
 Qed.
 
 Lemma lookup_update_neq : forall {A} (m : map A) k k' v,
@@ -34,93 +34,129 @@ Lemma lookup_update_neq : forall {A} (m : map A) k k' v,
   m[k' <== v] k = m k.
 Proof.
   intros. unfold update, update'.
-  destruct eqb eqn:E; trivial.
-  apply eqb_eq in E. contradiction.
+  destruct string_dec; trivial; subst. contradiction.
 Qed.
 
 (* ------------------------------------------------------------------------- *)
 (* Equivalence                                                               *)
 (* ------------------------------------------------------------------------- *)
 
-Definition equivalent {A} (m1 m2 : map A) :=
+Definition map_equivalence {A} (m1 m2 : map A) :=
   forall k, m1 k = m2 k.
 
-Lemma equivalent_refl : forall {A} (m1 m2 : map A),
-  equivalent m1 m2 ->
-  equivalent m2 m1.
-Proof.
-  unfold equivalent in *. intros. eauto.
-Qed.
+Notation " m1 === m2 " := (map_equivalence m1 m2)
+  (at level 70, no associativity).
 
-Lemma equivalent_trans : forall {A} (m1 m2 m3 : map A),
-  equivalent m1 m2 ->
-  equivalent m2 m3 ->
-  equivalent m1 m3.
-Proof.
-  unfold equivalent in *. intros * H ? *. rewrite H. eauto.
-Qed.
+Module MapEquivalence.
+  Lemma refl : forall {A} (m : map A),
+    m === m.
+  Proof.
+    unfold map_equivalence. intros. eauto.
+  Qed.
 
-Lemma equivalent_lookup : forall {A} (m1 m2 : map A) k v,
-  equivalent m1 m2 ->
-  m1 k = v ->
-  m2 k = v. 
-Proof.
-  intros * Heq ?. specialize (Heq k). inversion Heq. trivial.
-Qed.
+  Lemma trans : forall {A} (m1 m2 m3 : map A),
+    m1 === m2 ->
+    m2 === m3 ->
+    m1 === m3.
+  Proof.
+    unfold map_equivalence. intros * H1 H2 ?.
+    rewrite (H1 _). rewrite (H2 _). trivial.
+  Qed.
 
-Lemma equivalent_update : forall {A} (m1 m2 : map A) k v,
-  equivalent m1 m2 ->
-  equivalent m1[k <== v] m2[k <== v].
-Proof.
-  unfold equivalent, update, update'. intros. destruct eqb; eauto.
-Qed.
+  Lemma sym : forall {A} (m1 m2 : map A),
+    m1 === m2 ->
+    m2 === m1.
+  Proof.
+    unfold map_equivalence. intros. eauto.
+  Qed.
 
-Lemma equivalent_update_permutation : forall {A} (m : map A) k1 k2 v1 v2,
-  k1 <> k2 ->
-  equivalent m[k1 <== v1][k2 <== v2] m[k2 <== v2][k1 <== v1].
-Proof.
-  unfold equivalent, update, update'. intros.
-  destruct (eqb k1 k) eqn:E1; destruct (eqb k2 k) eqn:E2; auto.
-  apply eqb_eq in E1, E2. subst. contradiction.
-Qed.
+  Lemma lookup : forall {A} (m1 m2 : map A) k v,
+    m1 === m2 ->
+    m1 k = v ->
+    m2 k = v. 
+  Proof.
+    intros * Heq ?. specialize (Heq k). inversion Heq. trivial.
+  Qed.
 
-Lemma equivalent_update_overwrite : forall {A} (m : map A) k v v',
-  equivalent m[k <== v] m[k <== v'][k <== v].
-Proof.
-  unfold equivalent, update, update'. intros.
-  destruct eqb; intros; trivial.
-Qed.
+  Lemma update_equivalence : forall {A} (m1 m2 : map A) k v,
+    m1 === m2 ->
+    m1[k <== v] === m2[k <== v].
+  Proof.
+    unfold map_equivalence, update, update'. intros.
+    destruct string_dec; trivial.
+  Qed.
+
+  Lemma update_permutation : forall {A} (m : map A) k1 k2 v1 v2,
+    k1 <> k2 ->
+    m[k1 <== v1][k2 <== v2] === m[k2 <== v2][k1 <== v1].
+  Proof.
+    unfold map_equivalence, update, update'. intros.
+    do 2 (destruct string_dec; subst); trivial.
+    contradiction.
+  Qed.
+
+  Lemma update_overwrite : forall {A} (m : map A) k v v',
+    m[k <== v] === m[k <== v'][k <== v].
+  Proof.
+    unfold map_equivalence, update, update'. intros.
+    destruct string_dec; intros; trivial.
+  Qed.
+End MapEquivalence.
 
 (* ------------------------------------------------------------------------- *)
 (* Inclusion                                                                 *)
 (* ------------------------------------------------------------------------- *)
 
 (* m includes m' *)
-Definition includes' {A} (m m' : map A) := forall k v,
+Definition inclusion {A} (m m' : map A) := forall k v,
   m' k = Some v -> m k = Some v.
 
-Infix "includes" := includes' (at level 50, left associativity).
+Infix "includes" := inclusion (at level 70, no associativity).
 
-Lemma inclusion_update : forall {A} (m m' : map A) k v,
-  m includes m' ->
-  m[k <== v] includes m'[k <== v].
-Proof.
-  unfold includes', update, update'. intros. destruct eqb; auto.
-Qed.
+Module MapInclusion.
+  Lemma refl : forall {A} (m : map A),
+    m includes m.
+  Proof.
+    unfold inclusion. intros. eauto.
+  Qed.
 
-Lemma inclusion_update_permutation : forall {A} (m : map A) k1 k2 v1 v2,
-  k1 <> k2 ->
-  m[k1 <== v1][k2 <== v2] includes m[k2 <== v2][k1 <== v1].
-Proof.
-  unfold includes', update, update'. intros.
-  destruct (eqb k1 k) eqn:E1; destruct (eqb k2 k) eqn:E2; auto.
-  apply eqb_eq in E1, E2. subst. contradiction.
-Qed.
+  Lemma trans : forall {A} (m1 m2 m3 : map A),
+    m1 includes m2 ->
+    m2 includes m3 ->
+    m1 includes m3.
+  Proof.
+    unfold inclusion. intros * H1 H2 ? ? ?.
+    rewrite (H1 k v); trivial. rewrite (H2 k v); trivial.
+  Qed.
 
-Lemma inclusion_update_overwrite : forall {A} (m : map A) k v v',
-  m[k <== v] includes m[k <== v'][k <== v].
-Proof.
-  unfold includes', update, update'. intros.
-  destruct eqb; intros; assumption.
-Qed.
+  Lemma antisym : forall {A} (m1 m2 : map A),
+    m1 includes m2 ->
+    m2 includes m1 ->
+    m1 = m2.
+  Proof.
+  Abort.
+
+  Lemma update_inclusion : forall {A} (m m' : map A) k v,
+    m includes m' ->
+    m[k <== v] includes m'[k <== v].
+  Proof.
+    unfold inclusion, update, update'. intros.
+    destruct string_dec; eauto.
+  Qed.
+
+  Lemma update_permutation : forall {A} (m : map A) k1 k2 v1 v2,
+    k1 <> k2 ->
+    m[k1 <== v1][k2 <== v2] includes m[k2 <== v2][k1 <== v1].
+  Proof.
+    unfold inclusion, update, update'. intros.
+    do 2 (destruct string_dec; subst); trivial. contradiction.
+  Qed.
+
+  Lemma update_overwrite : forall {A} (m : map A) k v v',
+    m[k <== v] includes m[k <== v'][k <== v].
+  Proof.
+    unfold inclusion, update, update'. intros.
+    destruct string_dec; trivial.
+  Qed.
+End MapInclusion.
 
